coq/Frontend/ODMG/TOQL.v
@@ -19,7 +19,8 @@ Section TOQL.
   Require Import String.
   Require Import List.
   Require Import Arith.
-  Require Import EquivDec.
+  Require Import Program.
+  Require Import EquivDec Morphisms.
 
   Require Import Utils BasicSystem.
 
@@ -30,6 +31,7 @@ Section TOQL.
   Section typ.
   
     Context {m:basic_model}.
+    Context (τconstants:tbindings).
     Hint Resolve bindings_type_has_type.
 
     Inductive oql_expr_type : tbindings -> oql_expr -> rtype -> Prop :=
@@ -37,9 +39,33 @@ Section TOQL.
         data_type (normalize_data brand_relation_brands c) τ ->
         oql_expr_type tenv (OConst c) τ
     | OTVar {τ} tenv v :
-        lookup equiv_dec tenv v = Some τ -> oql_expr_type tenv (OVar v) τ
+        edot tenv v = Some τ -> oql_expr_type tenv (OVar v) τ
+    | OTTable {τ} tenv s :
+      tdot τconstants s = Some τ ->
+      oql_expr_type tenv (OTable s) τ
     .
+  End typ.
+    
+  (** Main typing soundness theorem for OQL *)
 
+  Theorem typed_oql_yields_typed_data {m:basic_model} {τc} {τenv τout} c (env:list (string*data)) (q:oql_expr):
+    bindings_type c τc ->
+    bindings_type env τenv ->
+    (oql_expr_type τc τenv q τout) ->
+    (exists x, (oql_interp brand_relation_brands c q env = Some x /\ (x ▹ τout))).
+  Proof.
+    intros.
+    revert c env H H0.
+    dependent induction H1; simpl; intros.
+    - exists (normalize_data brand_relation_brands c).
+      split; [reflexivity|assumption].
+    - unfold bindings_type in H1.
+      apply (Forall2_lookupr_some _ _ _ _ H1).
+      assumption.
+    - unfold bindings_type in H0.
+      apply (Forall2_lookupr_some _ _ _ _ H0).
+      assumption.
+  Qed.
   
 End TOQL.
 
